Flatten rules, make thread boundaries explicit

Atomics.thy
@@ -21,6 +21,9 @@ text \<open>Weakest precondition for a precondition and postrelation\<close>
 definition wp 
   where "wp pre post Q \<equiv> pre \<inter> {m. (\<forall>m'. (m,m') \<in> post \<longrightarrow> m' \<in> Q)}"
 
+definition guar
+  where "guar pre post G \<equiv> {(m,m'). m \<in> pre \<and> (m,m') \<in> post} \<subseteq> G"
+
 subsection \<open>Helper Lemmas\<close>
 
 lemma stable_conseqI [intro]:
@@ -58,8 +61,7 @@ text \<open>Weakest precondition of a program, only covering basic instructions,
 fun wp\<^sub>c :: "('a,'b) com \<Rightarrow> 'b pred \<Rightarrow> 'b pred"
   where 
     "wp\<^sub>c (Basic \<alpha>) Q = wp\<^sub>\<alpha> \<alpha> Q" |
-    "wp\<^sub>c (Rel r) Q = wp UNIV r Q" |
-    "wp\<^sub>c (c\<^sub>1 ; c\<^sub>2) Q = wp\<^sub>c c\<^sub>1 (wp\<^sub>c c\<^sub>2 Q)" |
+    "wp\<^sub>c (Seq c\<^sub>1 c\<^sub>2) Q = wp\<^sub>c c\<^sub>1 (wp\<^sub>c c\<^sub>2 Q)" |
     "wp\<^sub>c _ Q = undefined"
 
 text \<open>Refinement relation between two programs, in terms of their weakest precondition calculation.\<close>
@@ -71,15 +73,15 @@ definition eval :: "('a,'b) basic \<Rightarrow> 'b rel"
   where "eval \<alpha> \<equiv> {(m,m'). m \<in> vc \<alpha> \<longrightarrow> (m,m') \<in> beh \<alpha>}"
 
 text \<open>Specification check, ensuring an instruction conforms to a relation\<close>
-abbreviation guar :: "('a,'b) basic \<Rightarrow> 'b rpred \<Rightarrow> bool"
-  where "guar \<alpha> G \<equiv> {(m,m'). m \<in> vc \<alpha> \<and> (m,m') \<in> beh \<alpha>} \<subseteq> G\<^sup>="
+abbreviation guar\<^sub>\<alpha> :: "('a,'b) basic \<Rightarrow> 'b rpred \<Rightarrow> bool"
+  where "guar\<^sub>\<alpha> \<alpha> G \<equiv> guar (vc \<alpha>) (beh \<alpha>) G"
 
 section \<open>Atomic Rule\<close>
 
 text \<open>Rule for an atomic operation\<close>
 definition atomic_rule :: "'b rpred \<Rightarrow> 'b rpred \<Rightarrow> 'b pred \<Rightarrow> ('a,'b) basic \<Rightarrow> 'b pred \<Rightarrow> bool" 
   ("_,_ \<turnstile>\<^sub>A _ {_} _" [40,0,0,0,40] 40)
-  where "R,G \<turnstile>\<^sub>A P {\<alpha>} Q \<equiv> P \<subseteq> wp\<^sub>\<alpha> \<alpha> Q \<and> guar \<alpha> G \<and> stable R P \<and> stable R Q"
+  where "R,G \<turnstile>\<^sub>A P {\<alpha>} Q \<equiv> P \<subseteq> wp\<^sub>\<alpha> \<alpha> Q \<and> guar\<^sub>\<alpha> \<alpha> G \<and> stable R P \<and> stable R Q"
 
 subsection \<open>Derived Properties\<close>
 
@@ -93,7 +95,7 @@ text \<open>Strengthen the rely and weaken the guarantee for an atomic judgement
 lemma atomic_conseqI [intro]:
   assumes "R,G \<turnstile>\<^sub>A P {\<alpha>} Q" "R' \<subseteq> R" "G \<subseteq> G'"
   shows "R',G' \<turnstile>\<^sub>A P {\<alpha>} Q"
-  using assms unfolding atomic_rule_def by blast
+  using assms unfolding atomic_rule_def guar_def by blast
 
 text \<open>Atomic judgements over the same instruction can be combined\<close>
 lemma actomic_conjI [intro]:
@@ -110,14 +112,14 @@ lemma atomic_invI [intro]:
 proof (safe, goal_cases)
   case (1 m)
   hence "{(m,m'). m \<in> P \<inter> vc \<alpha> \<and> (m,m') \<in> beh \<alpha>} \<subseteq> R\<^sub>2\<^sup>=" "m \<in> vc \<alpha>"
-    using assms(1,3) by (auto simp: wp_def atomic_rule_def)
+    using assms(1,3) by (auto simp: wp_def guar_def atomic_rule_def)
   hence "m \<in> wp\<^sub>\<alpha> \<alpha> I" using assms(2) 1 by (auto simp: wp_def stable_def)
   moreover have "m \<in> wp\<^sub>\<alpha> \<alpha> Q" using 1 assms(1) by (auto simp: atomic_rule_def wp_def)
   ultimately show ?case by (auto simp: wp_def)
 qed (insert assms, auto simp: atomic_rule_def wp_def)
 
 lemma atomic_falseI [intro]:
-  assumes "guar \<beta> G"
+  assumes "guar\<^sub>\<alpha> \<beta> G"
   shows "R,G \<turnstile>\<^sub>A {} {\<beta>} {}"
   using assms unfolding atomic_rule_def by auto
 
@@ -151,10 +153,10 @@ lemma expand_wp\<^sub>\<alpha>:
   by fastforce
 
 lemma expand_guar:
-  assumes "guar \<alpha> G" "valid_expand m r"
+  assumes "guar\<^sub>\<alpha> \<alpha> G" "valid_expand m r"
   assumes \<alpha>: "vc \<alpha>' = expand\<^sub>P m (vc \<alpha>)" "beh \<alpha>' = expand\<^sub>G m r (beh \<alpha>)"
-  shows "guar \<alpha>' (expand\<^sub>G m r G)"
-  using assms(1,2,3) unfolding valid_expand_def expand\<^sub>G_def \<alpha> expand\<^sub>P_def
+  shows "guar\<^sub>\<alpha> \<alpha>' (expand\<^sub>G m r G)"
+  using assms(1,2,3) unfolding valid_expand_def expand\<^sub>G_def \<alpha> expand\<^sub>P_def guar_def
   by blast
 
 text \<open>Expand the state of an atomic judgement\<close>
@@ -175,10 +177,8 @@ next
   thus "x \<in> wp\<^sub>\<alpha> \<alpha>' (expand\<^sub>P m Q)"
     using assms(1,2) \<alpha> expand_wp\<^sub>\<alpha> unfolding atomic_rule_def by blast
 next
-  fix x x' assume b: "(x, x') \<notin> expand\<^sub>G m r G" "x \<in> vc \<alpha>'" "(x, x') \<in> beh \<alpha>'"
-  have "guar \<alpha>' (expand\<^sub>G m r G)"
+  show "guar\<^sub>\<alpha> \<alpha>' (expand\<^sub>G m r G)"
     using assms(1,2) \<alpha> expand_guar unfolding atomic_rule_def by blast
-  thus "x = x'" using b by auto
 qed
 
 section \<open>Auxiliary State\<close>
@@ -190,7 +190,7 @@ definition aux\<^sub>R
   where "aux\<^sub>R r R \<equiv> {(m,m'). \<forall>n. (m,n) \<in> r\<^sup>= \<longrightarrow> (\<exists>n'. (m',n') \<in> r\<^sup>= \<and> (n,n') \<in> R)}"
 
 definition aux\<^sub>G
-  where "aux\<^sub>G r R \<equiv> {(m,m'). \<exists>n n'. (m,n) \<in> r\<^sup>= \<and> (m',n') \<in> r\<^sup>= \<and> (n,n') \<in> R\<^sup>=}"
+  where "aux\<^sub>G r R \<equiv> {(m,m'). \<exists>n n'. (m,n) \<in> r\<^sup>= \<and> (m',n') \<in> r\<^sup>= \<and> (n,n') \<in> R}"
 
 lemma aux\<^sub>P_mono [intro]:
   "P \<subseteq> Q \<Longrightarrow> aux\<^sub>P a P \<subseteq> aux\<^sub>P a Q"
@@ -219,50 +219,50 @@ proof (clarsimp, goal_cases)
   then show ?case using a(1) by auto
 qed
 
+abbreviation aux\<^sub>\<alpha>
+  where "aux\<^sub>\<alpha> r \<alpha> \<equiv> (tag \<alpha>, aux\<^sub>P r (vc \<alpha>), aux\<^sub>R r (beh \<alpha>))"
+
 lemma aux_wp [intro]:
-  assumes "P \<subseteq> wp\<^sub>\<alpha> \<alpha> Q" "beh \<alpha>' = aux\<^sub>R r (beh \<alpha>)" "vc \<alpha>' = aux\<^sub>P r (vc \<alpha>)"
-  shows "aux\<^sub>P r P \<subseteq> wp\<^sub>\<alpha> \<alpha>' (aux\<^sub>P r Q)"
+  assumes "P \<subseteq> wp\<^sub>\<alpha> \<alpha> Q"
+  shows "aux\<^sub>P r P \<subseteq> wp\<^sub>\<alpha> (aux\<^sub>\<alpha> r \<alpha>) (aux\<^sub>P r Q)"
   unfolding wp_def aux\<^sub>P_def
 proof (clarsimp, (intro conjI; clarsimp), goal_cases)
   case (1 n m')
-  then show ?case using assms(1,3) by (auto simp: wp_def aux\<^sub>P_def)
+  then show ?case using assms by (auto simp: wp_def aux\<^sub>P_def)
 next
   case (2 n m n')
-  then show ?case using assms(1) unfolding assms(2) aux\<^sub>R_def wp_def by blast
+  then show ?case using assms(1) unfolding aux\<^sub>R_def wp_def by blast
 qed
 
 lemma aux_guar [intro]:
-  assumes "guar \<alpha> G" "beh \<alpha>' = aux\<^sub>R r (beh \<alpha>)" "vc \<alpha>' = aux\<^sub>P r (vc \<alpha>)"
-  shows "guar \<alpha>' (aux\<^sub>G r G)"
-  unfolding wp_def aux\<^sub>G_def assms(2,3) aux\<^sub>P_def aux\<^sub>R_def
-proof (clarify, goal_cases)
+  assumes "guar\<^sub>\<alpha> \<alpha> G" 
+  shows "guar\<^sub>\<alpha> (aux\<^sub>\<alpha> r \<alpha>) (aux\<^sub>G r G)"
+  unfolding wp_def aux\<^sub>G_def aux\<^sub>P_def aux\<^sub>R_def guar_def
+proof (clarsimp, goal_cases)
   case (1 m m' n)
   then obtain n' where a: "(m', n') \<in> r\<^sup>=" "(n, n') \<in> beh \<alpha>" by auto
-  hence "(n,n') \<in> G\<^sup>=" using assms(1) 1 by auto
-  thus ?case using a(1) 1(3) by blast
+  hence "(n,n') \<in> G" using assms 1 by (auto simp: guar_def)
+  thus ?case using a(1) 1(3) sorry
 qed
 
 lemma atomic_auxI [intro]:
   assumes "R,G \<turnstile>\<^sub>A P {\<alpha>} Q" 
-  assumes "beh \<alpha>' = aux\<^sub>R r (beh \<alpha>)"
-  assumes "vc \<alpha>' = aux\<^sub>P r (vc \<alpha>)"
-  shows "aux\<^sub>R r R,aux\<^sub>G r G \<turnstile>\<^sub>A aux\<^sub>P r P {\<alpha>'} aux\<^sub>P r Q"
+  shows "aux\<^sub>R r R,aux\<^sub>G r G \<turnstile>\<^sub>A aux\<^sub>P r P {aux\<^sub>\<alpha> r \<alpha>} aux\<^sub>P r Q"
   unfolding atomic_rule_def
 proof (intro conjI)
   show "stable (aux\<^sub>R r R) (aux\<^sub>P r P)" using assms(1) by (auto simp: atomic_rule_def)
 next
   show "stable (aux\<^sub>R r R) (aux\<^sub>P r Q)" using assms(1) by (auto simp: atomic_rule_def)
 next
-  have "guar \<alpha> G" using assms(1) by (auto simp: atomic_rule_def)
-  thus "guar \<alpha>' (aux\<^sub>G r G)" using aux_guar assms(2,3) by blast
+  have "guar\<^sub>\<alpha> \<alpha> G" using assms(1) by (auto simp: atomic_rule_def)
+  thus "guar\<^sub>\<alpha> (aux\<^sub>\<alpha> r \<alpha>) (aux\<^sub>G r G)" using aux_guar by blast
 next
   have "P \<subseteq> wp\<^sub>\<alpha> \<alpha> Q" using assms(1) by (auto simp: atomic_rule_def)
-  thus "aux\<^sub>P r P \<subseteq> wp\<^sub>\<alpha> \<alpha>' (aux\<^sub>P r Q)" using aux_wp assms(2,3) by blast
+  thus "aux\<^sub>P r P \<subseteq> wp\<^sub>\<alpha> (aux\<^sub>\<alpha> r \<alpha>) (aux\<^sub>P r Q)" using aux_wp by blast
 qed
 
-abbreviation aux\<^sub>\<alpha>
-  where "aux\<^sub>\<alpha> r \<alpha> \<equiv> (tag \<alpha>, aux\<^sub>P r (vc \<alpha>), aux\<^sub>R r (beh \<alpha>))"
 
+(*
 fun aux\<^sub>c
   where
     "aux\<^sub>c r Nil = Nil" |
@@ -272,7 +272,7 @@ fun aux\<^sub>c
     "aux\<^sub>c r (c\<^sub>1 \<sqinter> c\<^sub>2)  = (aux\<^sub>c r c\<^sub>1 \<sqinter> aux\<^sub>c r c\<^sub>2)" |
     "aux\<^sub>c r (Loop c) = Loop (aux\<^sub>c r c)" |
     "aux\<^sub>c r (BigChoice S\<^sub>1) = (BigChoice ((map (aux\<^sub>\<alpha> r)) ` S\<^sub>1))" |
-    "aux\<^sub>c r (Rel R) = Rel (aux\<^sub>R r R)" |
+    "aux\<^sub>c r (Dec b m c) = (Dec b m (aux\<^sub>c r c))" |
     "aux\<^sub>c r (c\<^sub>1 || c\<^sub>2) = (aux\<^sub>c r c\<^sub>1 || aux\<^sub>c r c\<^sub>2)"
 
 lemma aux\<^sub>c_nilE [elim!]:
@@ -310,5 +310,140 @@ lemma aux_local [intro]:
   assumes "local c" 
   shows "local (aux\<^sub>c r c)"
   using assms by (induct c rule: local.induct) auto
+*)
+
+(*
+lemma aux\<^sub>c_seqE2 [elim!]:
+  assumes "c\<^sub>1 ; c\<^sub>2 = aux\<^sub>c r c "
+  obtains c\<^sub>1' c\<^sub>2' where "c = c\<^sub>1' ; c\<^sub>2'" "aux\<^sub>c r c\<^sub>1' = c\<^sub>1" "aux\<^sub>c r c\<^sub>2' = c\<^sub>2"
+  using assms by (cases "(r,c)" rule: aux\<^sub>c.cases) auto
+
+lemma aux\<^sub>c_ordE [elim!]:
+  assumes "c\<^sub>1 \<cdot> c\<^sub>2 = aux\<^sub>c r c"
+  obtains c\<^sub>1' c\<^sub>2' where "c = c\<^sub>1' \<cdot> c\<^sub>2'" "aux\<^sub>c r c\<^sub>1' = c\<^sub>1" "aux\<^sub>c r c\<^sub>2' = c\<^sub>2"
+  using assms by (cases "(r,c)" rule: aux\<^sub>c.cases) auto
+
+lemma aux\<^sub>c_parE [elim!]:
+  assumes "c\<^sub>1 || c\<^sub>2 = aux\<^sub>c r c"
+  obtains c\<^sub>1' c\<^sub>2' where "c = c\<^sub>1' || c\<^sub>2'" "aux\<^sub>c r c\<^sub>1' = c\<^sub>1" "aux\<^sub>c r c\<^sub>2' = c\<^sub>2"
+  using assms by (cases "(r,c)" rule: aux\<^sub>c.cases) auto
+
+lemma aux\<^sub>c_choiceE [elim!]:
+  assumes "c\<^sub>1 \<sqinter> c\<^sub>2 = aux\<^sub>c r c"
+  obtains c\<^sub>1' c\<^sub>2' where "c = c\<^sub>1' \<sqinter> c\<^sub>2'" "aux\<^sub>c r c\<^sub>1' = c\<^sub>1" "aux\<^sub>c r c\<^sub>2' = c\<^sub>2"
+  using assms by (cases "(r,c)" rule: aux\<^sub>c.cases) auto
+
+lemma aux\<^sub>c_loopE [elim!]:
+  assumes "Loop c\<^sub>1 = aux\<^sub>c r c"
+  obtains c\<^sub>1' where "c = Loop c\<^sub>1'" "aux\<^sub>c r c\<^sub>1' = c\<^sub>1" 
+  using assms by (cases "(r,c)" rule: aux\<^sub>c.cases) auto
+
+lemma aux\<^sub>c_bigchoiceE [elim!]:
+  assumes "(\<Sqinter> S) = aux\<^sub>c r c"
+  obtains S' where "c = \<Sqinter> S'" "S = (map (aux\<^sub>\<alpha> r)) ` S'" 
+  using assms by (cases "(r,c)" rule: aux\<^sub>c.cases) auto
+
+lemma [simp]:
+  "seq2com (map (aux\<^sub>\<alpha> r) x) = aux\<^sub>c r (seq2com x)"
+proof (induct x)
+case Nil
+  then show ?case by auto
+next
+  case (Cons a x)
+  then show ?case  by auto
+qed
+
+lemma aux_rewriteE:
+  assumes "aux\<^sub>c r c \<leadsto> c\<^sub>a"
+  obtains c' where "c \<leadsto> c'" "aux\<^sub>c r c' = c\<^sub>a"
+  using assms
+  by (induct "aux\<^sub>c r c" c\<^sub>a arbitrary: r c) (auto; force)+
+
+lemma aux\<^sub>c_basicE [elim!]:
+  assumes "Basic \<alpha> = aux\<^sub>c r c"
+  obtains \<beta> where "c = Basic \<beta>" "\<alpha> = aux\<^sub>\<alpha> r \<beta>"
+  using assms by (cases "(r,c)" rule: aux\<^sub>c.cases) auto
+
+lemma [simp]:
+  "(aux\<^sub>\<alpha> r \<beta>)\<langle>tag x\<rangle> = aux\<^sub>\<alpha> r \<beta>\<langle>tag x\<rangle>"
+  
+  sorry
+
+lemma [simp]:
+  "(aux\<^sub>\<alpha> r \<beta>)\<llangle>aux\<^sub>c r p\<rrangle> = aux\<^sub>\<alpha> r \<beta>\<llangle>p\<rrangle>"
+  by (induct p arbitrary: \<beta>) auto
+
+lemma aux_re:
+  assumes "\<alpha>' < aux\<^sub>c r c <\<^sub>c aux\<^sub>\<alpha> r \<alpha>"
+  obtains \<beta> where "\<beta> < c <\<^sub>c \<alpha>" "\<alpha>' = aux\<^sub>\<alpha> r \<beta>"
+  using assms
+proof (induct c arbitrary: \<alpha>' \<alpha>)
+  case Nil
+  then show ?case by auto
+next
+  case (Basic x)
+  hence "tag x \<hookleftarrow> tag (\<alpha>)\<langle>tag x\<rangle>" by auto
+  moreover have "\<alpha>' = aux\<^sub>\<alpha> r \<alpha>\<langle>tag x\<rangle>" using Basic(2) by auto
+  ultimately show ?case using Basic(1) by auto
+next
+  case (Seq c1 c2)
+  then obtain \<beta> where b: "\<alpha>' < aux\<^sub>c r c1 <\<^sub>c \<beta>" "\<beta> < aux\<^sub>c r c2 <\<^sub>c aux\<^sub>\<alpha> r \<alpha>" by auto
+  show ?case 
+  proof (rule Seq(2)[OF _ b(2)])
+    fix \<beta>' assume c: "\<beta>' < c2 <\<^sub>c \<alpha>" "\<beta> = aux\<^sub>\<alpha> r \<beta>'"
+    hence a: "\<alpha>' < aux\<^sub>c r c1 <\<^sub>c aux\<^sub>\<alpha> r \<beta>'" using b by auto
+    show ?thesis apply (rule Seq(1)[OF _a]) using c(1) Seq(3) reorder_com.simps(3) by blast 
+  qed
+next
+  case (Ord c1 c2)
+  then obtain \<beta> where b: "\<alpha>' < aux\<^sub>c r c1 <\<^sub>c \<beta>" "\<beta> < aux\<^sub>c r c2 <\<^sub>c aux\<^sub>\<alpha> r \<alpha>" by auto
+  show ?case 
+  proof (rule Ord(2)[OF _ b(2)])
+    fix \<beta>' assume c: "\<beta>' < c2 <\<^sub>c \<alpha>" "\<beta> = aux\<^sub>\<alpha> r \<beta>'"
+    hence a: "\<alpha>' < aux\<^sub>c r c1 <\<^sub>c aux\<^sub>\<alpha> r \<beta>'" using b by auto
+    show ?thesis apply (rule Ord(1)[OF _a]) using c(1) Ord(3) reorder_com.simps(4) by blast 
+  qed
+qed auto
+
+lemma aux_execE:
+  assumes "aux\<^sub>c r c \<mapsto>[p,\<alpha>] c\<^sub>a"
+  obtains c' p' \<beta> where "c \<mapsto>[p',\<beta>] c'" "aux\<^sub>c r c' = c\<^sub>a" "\<alpha> = aux\<^sub>\<alpha> r \<beta>" "aux\<^sub>c r p' = p"
+  using assms
+proof (induct "aux\<^sub>c r c" p \<alpha> c\<^sub>a arbitrary: r c)
+  case (act \<alpha>)
+  then show ?case apply auto by force
+next
+  case (seq c\<^sub>1 r' \<alpha> c\<^sub>1' c\<^sub>2)
+  then show ?case apply auto by force
+next
+  case (ord c\<^sub>1 r \<alpha> c\<^sub>1' c\<^sub>2)
+  then show ?case apply auto by force
+next
+  case (ooo c\<^sub>2 r' \<alpha> c\<^sub>2' \<alpha>' c\<^sub>1)
+  then obtain c\<^sub>1' c' where s: "c = c\<^sub>1' ; c'" "c\<^sub>1 = aux\<^sub>c r c\<^sub>1'" "aux\<^sub>c r c' = c\<^sub>2" by auto
+
+  
+  show ?case 
+  proof (rule ooo(2)[of r c'], goal_cases)
+    case 1
+    then show ?case using s by auto
+  next
+    case (2 p' \<beta> c'')
+    hence re: "\<alpha>' < aux\<^sub>c r (c\<^sub>1' ; p') <\<^sub>c aux\<^sub>\<alpha> r \<beta>" using ooo(3) s by auto
+    then obtain \<beta>' where b: "\<beta>' < c\<^sub>1' ; p' <\<^sub>c \<beta>" using aux_re by blast
+
+    show ?case 
+      apply (rule ooo(5)[of "c\<^sub>1' ; p'" \<beta> "c\<^sub>1' ; c''"])
+      using s 2 b apply auto
+      apply (rule execute.ooo[of _ _ _ _ \<beta>'], simp)
+      by auto
+  qed 
+next
+  case (par1 c\<^sub>1 r' \<alpha> c\<^sub>1' c\<^sub>2)
+  then show ?case apply auto by force
+next
+  case (par2 c\<^sub>2 r' \<alpha> c\<^sub>2' c\<^sub>1)
+  then show ?case apply auto by force
+qed *)
 
 end
