Syntax.thy
@@ -26,23 +26,19 @@ datatype ('a,'b) com =
   | Basic "('a,'b) basic"
   | Seq "('a,'b) com" "('a,'b) com" (infixr ";" 80)
   | Ord "('a,'b) com" "('a,'b) com" (infixr "\<cdot>" 80)
-  | BigChoice "('a,'b) seq set" ("\<Sqinter> _" 150)
+  | SeqChoice "('a,'b) seq set" ("\<Sqinter> _" 150)
   | Choice "('a,'b) com" "('a,'b) com" (infixr "\<sqinter>" 150)
   | Loop "('a,'b) com" ("_*" [100] 150)
   | Parallel "('a,'b) com" "('a,'b) com"  (infixr "||" 150)
-  | Rel "'b rel"
-
-text \<open>Convert a sequence to a command\<close>
-fun seq2com
-  where "seq2com [] = Nil" | "seq2com (\<alpha>#t) = Basic \<alpha> \<cdot> seq2com t"
+  | Thread 'b "'b \<Rightarrow> 'b \<Rightarrow> 'b" "('a,'b) com"
 
 text \<open>Ensure there is no parallelism within a program\<close>
 fun local :: "('a,'b) com \<Rightarrow> bool"
   where 
     "local (c\<^sub>1 || c\<^sub>2) = False" |
-    "local (Rel r) = False" |
-    "local (c\<^sub>1 ; c\<^sub>2) = (local c\<^sub>1 \<and> local c\<^sub>2)" |    
-    "local (c\<^sub>1 \<cdot> c\<^sub>2) = (local c\<^sub>1 \<and> local c\<^sub>2)" |    
+    "local (Thread _ _ _) = False" |
+    "local (c\<^sub>1 ; c\<^sub>2) = (local c\<^sub>1 \<and> local c\<^sub>2)" |
+    "local (c\<^sub>1 \<cdot> c\<^sub>2) = (local c\<^sub>1 \<and> local c\<^sub>2)" |        
     "local (c\<^sub>1 \<sqinter> c\<^sub>2) = (local c\<^sub>1 \<and> local c\<^sub>2)" |  
     "local (c*) = (local c)" |    
     "local _ = True"
@@ -54,12 +50,28 @@ fun basics :: "('a,'b) com \<Rightarrow> ('a,'b) basic set"
     "basics (Seq c\<^sub>1 c\<^sub>2) = basics c\<^sub>1 \<union> basics c\<^sub>2" |
     "basics (Ord c\<^sub>1 c\<^sub>2) = basics c\<^sub>1 \<union> basics c\<^sub>2" |
     "basics (Choice c\<^sub>1 c\<^sub>2) = basics c\<^sub>1 \<union> basics c\<^sub>2" |
-    "basics (BigChoice S) = (\<Union>s \<in> S. set s)" |
+    "basics (SeqChoice S) = (\<Union>s \<in> S. set s)" |
     "basics (Parallel c\<^sub>1 c\<^sub>2) = basics c\<^sub>1 \<union> basics c\<^sub>2" |
     "basics (Loop c) = basics c" |
+    "basics (Thread _ _ c) = basics c" |
     "basics _ = {}"
 
+fun compare :: "(('a,'b) basic \<Rightarrow> ('a,'b) basic \<Rightarrow> bool) \<Rightarrow> ('a,'b) com \<Rightarrow> ('a,'b) com \<Rightarrow> bool"
+  where
+    "compare T Nil Nil = True" |
+    "compare T (Basic \<alpha>) (Basic \<beta>) = (T \<alpha> \<beta>)" |
+    "compare T (Seq c\<^sub>1 c\<^sub>2) (Seq c\<^sub>1' c\<^sub>2') = (compare T c\<^sub>1 c\<^sub>1' \<and> compare T c\<^sub>2 c\<^sub>2')" |
+    "compare T (Ord c\<^sub>1 c\<^sub>2) (Ord c\<^sub>1' c\<^sub>2') = (compare T c\<^sub>1 c\<^sub>1' \<and> compare T c\<^sub>2 c\<^sub>2')" |
+    "compare T (c\<^sub>1 \<sqinter> c\<^sub>2) (c\<^sub>1' \<sqinter> c\<^sub>2') = (compare T c\<^sub>1 c\<^sub>1' \<and> compare T c\<^sub>2 c\<^sub>2')" |
+    "compare T (Loop c) (Loop c') = (compare T c c')" |
+    "compare T (Thread s m c) (Thread s' m' c') = (compare T c c')" |
+    "compare _ _ _ = False"
+
 abbreviation Env
-  where "Env R \<equiv> Rel (R\<^sup>*)"
+  where "Env R \<equiv> Basic (undefined,UNIV,R\<^sup>*)"
+
+text \<open>Convert a sequence to a command\<close>
+fun seq2com
+  where "seq2com [] = Nil" | "seq2com (\<alpha>#t) = Basic \<alpha> \<cdot> seq2com t"
 
 end
