Rules.thy
@@ -1,0 +1,131 @@
+theory Rules
+  imports Interference
+begin
+
+chapter \<open>Rules\<close>
+
+text \<open>Define the rely/guarantee rules for a concurrent program.\<close>
+
+locale rules = interference
+
+context rules
+begin
+
+section \<open>Global Rules\<close>
+
+definition thr\<^sub>P
+  where "thr\<^sub>P op l P \<equiv> {m. op m l \<in> P}"
+
+definition thr\<^sub>G
+  where "thr\<^sub>G op G \<equiv> {(m,m') |m m' l l'. (op m l,op m' l') \<in> G}"
+
+definition thr\<^sub>R
+  where "thr\<^sub>R op R \<equiv> {(m,m') |m m'. \<forall>l. (op m l,op m' l) \<in> R}"
+
+lemma thr\<^sub>P_mono:
+  "P \<subseteq> Q \<Longrightarrow> thr\<^sub>P op l P \<subseteq> thr\<^sub>P op l Q"
+  unfolding thr\<^sub>P_def by auto
+
+lemma thr\<^sub>P_stable:
+  "stable R P \<Longrightarrow> stable (thr\<^sub>R op R) (thr\<^sub>P op l P)"
+  unfolding thr\<^sub>P_def thr\<^sub>R_def stable_def by auto
+
+text \<open>Establish the rules of the logic, similar to standard Hoare-logic\<close>
+inductive rules :: "'b rpred \<Rightarrow> 'b rpred \<Rightarrow> 'b set \<Rightarrow> ('a,'b) com \<Rightarrow> 'b set \<Rightarrow> bool" 
+  ("_,_ \<turnstile> _ {_} _" [69,0,0,0,69] 69)
+where
+  basic[intro]:  "R,G \<turnstile>\<^sub>A P {\<alpha>} Q \<Longrightarrow> R,G \<turnstile> P { Basic \<alpha> } Q" |
+  nil[intro]:    "stable R P \<Longrightarrow> R,G \<turnstile> P { Nil } P" |
+  seq[intro]:    "R,G \<turnstile> P { c\<^sub>1 } Q \<Longrightarrow> R,G \<turnstile> Q { c\<^sub>2 } M \<Longrightarrow> R,G \<turnstile> P { c\<^sub>1 ; c\<^sub>2 } M" |
+  ord[intro]:    "R,G \<turnstile> P { c\<^sub>1 } Q \<Longrightarrow> R,G \<turnstile> Q { c\<^sub>2 } M \<Longrightarrow> R,G \<turnstile> P { c\<^sub>1 \<cdot> c\<^sub>2 } M" |
+  choice[intro]: "R,G \<turnstile> P { c\<^sub>1 } Q \<Longrightarrow> R,G \<turnstile> P { c\<^sub>2 } Q \<Longrightarrow> R,G \<turnstile> P { c\<^sub>1 \<sqinter> c\<^sub>2 } Q" |
+  seqset[intro]: "\<forall>s \<in> S. R,G \<turnstile> P { seq2com s } Q \<Longrightarrow> R,G \<turnstile> P { \<Sqinter> S } Q" |
+  loop[intro]:   "stable R P \<Longrightarrow> R,G \<turnstile> P { c } P \<Longrightarrow> R,G \<turnstile> P { c* } P" |
+  thread[intro]: "R,G \<turnstile> P { c } Q \<Longrightarrow> inter R G c \<Longrightarrow> thr\<^sub>R op R,thr\<^sub>G op G \<turnstile> thr\<^sub>P op l P { Thread l op c } Q" |
+  par[intro]:    "R\<^sub>1,G\<^sub>1 \<turnstile> P\<^sub>1 { c\<^sub>1 } Q\<^sub>1 \<Longrightarrow> R\<^sub>2,G\<^sub>2 \<turnstile> P\<^sub>2 { c\<^sub>2 } Q\<^sub>2 \<Longrightarrow> G\<^sub>2 \<subseteq> R\<^sub>1 \<Longrightarrow> G\<^sub>1 \<subseteq> R\<^sub>2 \<Longrightarrow> 
+                  R\<^sub>1 \<inter> R\<^sub>2,G\<^sub>1 \<union> G\<^sub>2 \<turnstile> P\<^sub>1 \<inter> P\<^sub>2 { c\<^sub>1 || c\<^sub>2 } (Q\<^sub>1 \<inter> Q\<^sub>2)" |
+  conseq[intro]: "R,G \<turnstile> P { c } Q \<Longrightarrow> P' \<subseteq> P \<Longrightarrow> R' \<subseteq> R \<Longrightarrow> G \<subseteq> G' \<Longrightarrow> Q \<subseteq> Q' \<Longrightarrow> 
+                  R',G' \<turnstile> P' { c } Q'"  |
+  inv[intro]:    "R,G \<turnstile> P {c} Q \<Longrightarrow> stable R' I \<Longrightarrow> G \<subseteq> R' \<Longrightarrow> R \<inter> R',G \<turnstile> (P \<inter> I) {c} (Q \<inter> I)" 
+
+subsection \<open>Properties\<close>
+
+lemma nilE [elim!]:
+  assumes "R,G \<turnstile> P {Nil} Q"
+  obtains M where "stable R M" "P \<subseteq> M" "M \<subseteq> Q"
+  using assms by (induct R G P "Nil :: ('a,'b) com" Q) blast+
+
+lemma basicE [elim!]:
+  assumes "R,G \<turnstile> P {Basic \<beta>} Q"
+  obtains P' Q' where "P \<subseteq> P'" "R,G \<turnstile>\<^sub>A P' {\<beta>} Q'" "Q' \<subseteq> Q"
+  using assms 
+proof (induct R G P "Basic \<beta> :: ('a,'b) com" Q arbitrary: \<beta>)
+  case (basic R G P Q)
+  then show ?case by auto
+next
+  case (conseq R G P Q P' R' G' Q')
+  then show ?case using order.trans atomic_conseqI by metis
+next
+  case (inv R G P Q R' I)
+  show ?case 
+  proof (rule inv(2), goal_cases)
+    case (1 P' Q')
+    thus ?case using inv(3,4) inv(5)[of "P' \<inter> I" "Q' \<inter> I"] atomic_invI by blast
+  qed
+qed
+
+lemma seqE [elim]:
+  assumes "R,G \<turnstile> P {c\<^sub>1 ; c\<^sub>2} Q"
+  obtains M  where "R,G \<turnstile> P {c\<^sub>1} M" "R,G \<turnstile> M {c\<^sub>2} Q"
+  using assms 
+  by (induct R G P "c\<^sub>1 ; c\<^sub>2" Q arbitrary: c\<^sub>1 c\<^sub>2) blast+ 
+
+lemma ordE [elim]:
+  assumes "R,G \<turnstile> P {c\<^sub>1 \<cdot> c\<^sub>2} Q"
+  obtains M  where "R,G \<turnstile> P {c\<^sub>1} M" "R,G \<turnstile> M {c\<^sub>2} Q"
+  using assms 
+  by (induct R G P "c\<^sub>1 \<cdot> c\<^sub>2" Q arbitrary: c\<^sub>1 c\<^sub>2) blast+
+
+lemma stable_preE:
+  assumes "R,G \<turnstile> P {c} Q"
+  shows "\<exists>P'. P \<subseteq> P' \<and> stable R P' \<and> R,G \<turnstile> P' {c} Q"
+  using assms 
+proof (induct)
+  case (thread R G P c Q op l)
+  then show ?case by (metis thr\<^sub>P_stable thr\<^sub>P_mono rules.thread)
+next 
+  case (par R\<^sub>1 G\<^sub>1 P\<^sub>1 c\<^sub>1 Q\<^sub>1 R\<^sub>2 G\<^sub>2 P\<^sub>2 c\<^sub>2 Q\<^sub>2)
+  obtain P\<^sub>1' where 1: "P\<^sub>1 \<subseteq> P\<^sub>1'" "stable R\<^sub>1 P\<^sub>1'" "R\<^sub>1,G\<^sub>1 \<turnstile> P\<^sub>1' {c\<^sub>1} Q\<^sub>1" using par by auto
+  obtain P\<^sub>2' where 2: "P\<^sub>2 \<subseteq> P\<^sub>2'" "stable R\<^sub>2 P\<^sub>2'" "R\<^sub>2,G\<^sub>2 \<turnstile> P\<^sub>2' {c\<^sub>2} Q\<^sub>2" using par by auto
+  hence "R\<^sub>1 \<inter> R\<^sub>2,G\<^sub>1 \<union> G\<^sub>2 \<turnstile> P\<^sub>1' \<inter> P\<^sub>2' {c\<^sub>1 || c\<^sub>2} Q\<^sub>1 \<inter> Q\<^sub>2" using 1 2 rules.par par(5,6) by simp
+  thus ?case using 1 2 stable_conjI by blast
+next
+  case (basic R G P \<alpha> Q)
+  then show ?case using atomic_rule_def by fast
+next
+  case (choice R G P c\<^sub>1 Q c\<^sub>2)
+  obtain P\<^sub>1 where 1: "P \<subseteq> P\<^sub>1" "stable R P\<^sub>1" "R,G \<turnstile> P\<^sub>1 {c\<^sub>1} Q" using choice by auto
+  obtain P\<^sub>2 where 2: "P \<subseteq> P\<^sub>2" "stable R P\<^sub>2" "R,G \<turnstile> P\<^sub>2 {c\<^sub>2} Q" using choice by auto
+  have "stable R (P\<^sub>1 \<inter> P\<^sub>2)" using 1 2 by auto
+  thus ?case using 1 2 by blast
+next
+  case (seqset S R G P Q)
+  hence "\<exists>P\<^sub>s. \<forall>s\<in>S. P \<subseteq> P\<^sub>s s \<and> stable R (P\<^sub>s s) \<and> (R,G \<turnstile> P\<^sub>s s {seq2com s} Q)"
+    by metis
+  then obtain P\<^sub>s where s: "\<forall>s\<in>S. P \<subseteq> P\<^sub>s s \<and> stable R (P\<^sub>s s) \<and> (R,G \<turnstile> P\<^sub>s s {seq2com s} Q)"
+    by blast
+  hence "stable R (\<Inter>s\<in>S. P\<^sub>s s)" by (auto simp: stable_def)
+  moreover have "P \<subseteq> (\<Inter>s\<in>S. P\<^sub>s s)" using s by auto
+  ultimately show ?case using s seqset.hyps(1) by blast
+next
+  case (conseq R G P c Q P' R' G' Q')
+  then show ?case by (meson order_refl rules.conseq stable_conseqI subset_trans)
+next
+  case (inv R G P c Q R' I)
+  then obtain P' where "P \<subseteq> P'" "stable R P'" "R,G \<turnstile> P' {c} Q" by auto
+  then show ?case using inv rules.inv by blast
+qed blast+
+
+end
+
+end
